Add inv for fin type

eval.v
@@ -9,7 +9,7 @@ Unset Printing Implicit Defensive.
 (* An attempt at mechanizing Nbe *)
 
 Inductive Domain (n : nat) : Type :=
-| D_Clos m : tm (S m) -> (fin m -> Domain n) -> Domain n
+| D_Clos m : ty -> tm (S m) -> (fin m -> Domain n) -> Domain n
 | D_Ne (e : DomainNe n) : Domain n
 with DomainNe (n : nat) : Type :=
 | DN_var (i : fin n) : DomainNe n
@@ -22,13 +22,76 @@ Definition Env n m := fin n -> Domain m.
 Inductive D_Ap {n} : Domain n -> Domain n -> Domain n -> Prop :=
 | DAp_AppNeu e d :
   D_Ap (D_Ne e) d (D_Ne (DN_App e d))
-| DAp_App m a (ρ : Env m n) d0 d1 :
+| DAp_App m a A (ρ : Env m n) d0 d1 :
   D_Eval (d0 .: ρ) a d1 ->
-  D_Ap (D_Clos a ρ) d0 d1
+  D_Ap (D_Clos A a ρ) d0 d1
 with D_Eval {n} : forall {m}, Env m n -> tm m -> Domain n -> Prop :=
-| DEval_Abs m A a (ρ : Env m n) : D_Eval ρ (Lam A a) (D_Clos a ρ)
+| DEval_Var m (i : fin m) ρ : D_Eval ρ (var_tm i) (ρ i)
+| DEval_Abs m A a (ρ : Env m n) : D_Eval ρ (Lam A a) (D_Clos A a ρ)
 | DEval_App m a b d0 d1 d2 (ρ : Env m n) :
   D_Eval ρ a d0 ->
   D_Eval ρ b d1 ->
   D_Ap d0 d1 d2 ->
   D_Eval ρ (App a b) d2.
+
+Definition embed {n} : fin n -> fin (S n).
+  elim : n => [//|/= n embed].
+  case => [m | ].
+  - exact (Some (embed m)).
+  - exact None.
+Defined.
+
+Definition max_fin {n} : fin (S n).
+  elim : n => [//|n max_fin].
+  - exact None.
+  - exact (Some max_fin).
+Defined.
+
+(* Need the inv operation to define read back  *)
+Definition inv {n} (m : fin n) : fin n.
+  elim : n m => /= [// | n inv].
+  case => [m|].
+  - exact (embed (inv m)).
+  - exact max_fin.
+Defined.
+
+(* Need to show that inv is idempotent for the correctness proof  *)
+Lemma inv_embed_commute {n} (m : fin n) : Some (inv m) = inv (embed m).
+Proof.
+  elim : n m => [//| n ih m].
+  simpl in m.
+  case : m.
+  - hauto lq:on.
+  - reflexivity.
+Qed.
+
+Lemma inv_max_zero n : inv (@max_fin n) = None.
+Proof.
+  elim : n; hauto lq:on.
+Qed.
+
+Lemma inv_idempotent {n} (m : fin n) : inv (inv m) = m.
+Proof.
+  elim : n m => [// | n ihm m].
+  simpl in m.
+  case : m => [a|].
+  - hauto lq:on use:inv_embed_commute.
+  - sfirstorder use:inv_max_zero.
+Qed.
+
+
+(* TODO: add ren_domain? *)
+Inductive Readback {n} : Domain n -> tm n -> Prop :=
+| R_Clos m (ρ : Env m n) (a : tm (S m)) d A b:
+  D_Eval (D_Ne (DN_var (@max_fin)) .: ρ) a d ->
+  @Readback (S n) d b ->
+  Readback (D_Clos A a ρ : Domain n) (Lam A b : tm n)
+| R_Ne e a :
+  ReadbackNe e a ->
+  Readback (D_Ne e) a
+with ReadbackNe {n} : DomainNe n -> tm n -> Prop :=
+| R_Var i : ReadbackNe (DN_var i) (var_tm (inv i))
+| R_App e d a b :
+  ReadbackNe e a ->
+  Readback d b ->
+  ReadbackNe (DN_App e d) (App a b).
